% Options for packages loaded elsewhere
\PassOptionsToPackage{unicode}{hyperref}
\PassOptionsToPackage{hyphens}{url}
%
\documentclass[
]{article}
\usepackage{lmodern}
\usepackage{amssymb,amsmath}
\usepackage{ifxetex,ifluatex}
\ifnum 0\ifxetex 1\fi\ifluatex 1\fi=0 % if pdftex
  \usepackage[T1]{fontenc}
  \usepackage[utf8]{inputenc}
  \usepackage{textcomp} % provide euro and other symbols
\else % if luatex or xetex
  \usepackage{unicode-math}
  \defaultfontfeatures{Scale=MatchLowercase}
  \defaultfontfeatures[\rmfamily]{Ligatures=TeX,Scale=1}
\fi
% Use upquote if available, for straight quotes in verbatim environments
\IfFileExists{upquote.sty}{\usepackage{upquote}}{}
\IfFileExists{microtype.sty}{% use microtype if available
  \usepackage[]{microtype}
  \UseMicrotypeSet[protrusion]{basicmath} % disable protrusion for tt fonts
}{}
\makeatletter
\@ifundefined{KOMAClassName}{% if non-KOMA class
  \IfFileExists{parskip.sty}{%
    \usepackage{parskip}
  }{% else
    \setlength{\parindent}{0pt}
    \setlength{\parskip}{6pt plus 2pt minus 1pt}}
}{% if KOMA class
  \KOMAoptions{parskip=half}}
\makeatother
\usepackage{xcolor}
\IfFileExists{xurl.sty}{\usepackage{xurl}}{} % add URL line breaks if available
\IfFileExists{bookmark.sty}{\usepackage{bookmark}}{\usepackage{hyperref}}
\hypersetup{
  pdftitle={R Notebook},
  hidelinks,
  pdfcreator={LaTeX via pandoc}}
\urlstyle{same} % disable monospaced font for URLs
\usepackage[margin=1in]{geometry}
\usepackage{graphicx,grffile}
\makeatletter
\def\maxwidth{\ifdim\Gin@nat@width>\linewidth\linewidth\else\Gin@nat@width\fi}
\def\maxheight{\ifdim\Gin@nat@height>\textheight\textheight\else\Gin@nat@height\fi}
\makeatother
% Scale images if necessary, so that they will not overflow the page
% margins by default, and it is still possible to overwrite the defaults
% using explicit options in \includegraphics[width, height, ...]{}
\setkeys{Gin}{width=\maxwidth,height=\maxheight,keepaspectratio}
% Set default figure placement to htbp
\makeatletter
\def\fps@figure{htbp}
\makeatother
\setlength{\emergencystretch}{3em} % prevent overfull lines
\providecommand{\tightlist}{%
  \setlength{\itemsep}{0pt}\setlength{\parskip}{0pt}}
\setcounter{secnumdepth}{-\maxdimen} % remove section numbering

\title{R Notebook}
\author{}
\date{\vspace{-2.5em}}

\begin{document}
\maketitle

Since \(\text{E}_{\text{old}}\log p(\gamma|\phi^{\text{old}}, y)\) is a
constant to \(\phi\), we have \begin{align*}
&\quad \text{argmax}_{\phi}\text{E}_{\text{old}}\log p(\gamma|\phi, y) \\
&= \text{argmin}_{\phi}-\text{E}_{\text{old}}\log p(\gamma|\phi, y) \\
&= \text{argmin}_{\phi}\left\{\text{E}_{\text{old}}(-\log p(\gamma|\phi, y) + \log p(\gamma|\phi^{\text{old}}, y)) \right\}\\
&=\text{argmin}_{\phi}\text{E}_{\text{old}}\log \frac{p(\gamma|\phi^{\text{old}}, y)}{ p(\gamma|\phi, y)}.
\end{align*} So it is equivalent to minimizing \[
\text{E}_{\text{old}}\log \frac{p(\gamma|\phi^{\text{old}}, y)}{ p(\gamma|\phi, y)},
\] the KL divergence between \(p(\gamma|\phi^{\text{old}}, y)\) and
\(p(\gamma|\phi, y)\). Since \(-\log(x)\) is convex, by Jensen's
inequality we have \begin{align*}
\text{E}_{\text{old}}\log \frac{p(\gamma|\phi^{\text{old}}, y)}{ p(\gamma|\phi, y)} &= \text{E}_{\text{old}}-\log \frac{ p(\gamma|\phi, y)}{p(\gamma|\phi^{\text{old}}, y)}\\
&\geq -\log\text{E}_{\text{old}} \frac{ p(\gamma|\phi, y)}{p(\gamma|\phi^{\text{old}}, y)}\\
&= -\log(1) = 0.
\end{align*} The minimum \(0\) is achieved when
\(\phi = \phi^{\text{old}}\), because if \(\phi = \phi^{\text{old}}\)
then
\[\text{E}_{\text{old}}\log \frac{p(\gamma|\phi^{\text{old}}, y)}{ p(\gamma|\phi, y)} = \text{E}_{\text{old}}\log (1) = 0.\]
This proves that the maximizer of
\(\text{E}_{\text{old}}\log p(\gamma|\phi, y)\) is
\(\phi^{\text{old}}.\)

\hypertarget{problem-2}{%
\section{Problem 2}\label{problem-2}}

The log posterior is \begin{align*}
\ell &= \log p(\theta, \mu, \log\sigma, \log\tau | y) \\
&= -n \log\sigma - (J-1)\log\tau - \frac{1}{2\tau^2}\sum_{j=1}^{J}(\theta_j-\mu)^2 - \frac{1}{2\sigma^2}\sum_{j=1}^{J}\sum_{i=1}^{n_j}(y_{ij}-\theta_j)^2 + \text{constant.}
\end{align*} Taking derivative of with respect to \(\mu\) we have \[
\frac{\partial \text{E}_{\text{old}}\ell}{\partial \mu} = \frac{1}{\tau^2}\sum_{j=1}^{J}\text{E}_{\text{old}}(\theta_j-\mu).
\] Also, the second order derivative is negative (formula omitted).
Setting the derivative to be \(0\) we have
\(\mu^{\text{new}} = \frac{1}{J}\sum_{j=1}^{J}\hat{\theta}_j\).

Similarly,

\$\$ \frac{\partial \text{E}_{\text{old}}\ell}{\partial \sigma} =
-\frac{n}{\sigma} + \frac{1}{\sigma^3}
\sum\emph{\{j=1\}\^{}\{J\}\sum}\{i=1\}\^{}\{n\_j\}\text{E}\emph{\{\text{old}\}(y}\{ij\}-\theta\_j)\^{}2,

\[
and
\]
\frac{\partial \text{E}_{\text{old}}\ell}{\partial \sigma}\Big\rvert\emph{\{\mu =
\mu\^{}\{\text{new}\}\} = -\frac{J-1}{\tau} + \frac{1}{\tau^3}
\sum}\{j=1\}\^{}\{J\}\text{E}\_\{\text{old}\}(\theta\_j-\mu\textsuperscript{\{\text{new}\})}2.
\$\$

Setting the derivatives to be \(0\) we have \[
\sigma^{\text{new}} = \left(\frac{1}{n}\sum_{j=1}^{J}\sum_{i=1}^{n_j}\text{E}_{\text{old}}(y_{ij}-\theta_j)^2 \right)^{1/2} = \left(\frac{1}{n}\sum_{j=1}^{J}\sum_{i=1}^{n_j}\left((y_{ij}-\hat{\theta}_j)^2 + V_{\theta_j}\right) \right)^{1/2},
\] and \[
\tau^{\text{new}} =\left(\frac{1}{J-1}\sum_{j=1}^{J}\text{E}_{\text{old}}(\theta_j-\mu^{\text{new}})^2 \right)^{1/2} = \left(\frac{1}{J-1}\sum_{j=1}^{J}\left((\hat{\theta}_j - \mu^{\text{new}})^2 + V_{\theta_j}\right) \right)^{1/2}.
\]

\end{document}
